start the double induction (actually don't induct on rev of list for PRF)? need to manipulate the list properly to apply IH, but base cases look true! some clever IH constraints happening (calls >= i e.g.)

src/examples/HMAC_DRBG_nonadaptive.v
@@ -1899,7 +1899,7 @@ Definition bitsCallsKVeq_RB {A B : Type} (l1 l2 l : list B) (i : nat) (k_f k_oc 
   /\ l = l1 ++ l2 /\ length l1 = calls_prg /\ i < length l2.
 
 (* new postcondition *)
-Definition bitsCallsVEq {A B : Type} (l : list B) (calls i : nat)
+Definition bitsVEq {A B : Type} (l : list B) (i : nat)
            (x : A * (nat * KV)) (y : A * (nat * KV) * unit) :=
   let (bits_x, state_x) := x in
   let (calls_x, kv_x) := state_x in
@@ -1909,7 +1909,207 @@ Definition bitsCallsVEq {A B : Type} (l : list B) (calls i : nat)
   let (calls_y, kv_y) := state_y in
   let (k_y, v_y) := kv_y in
   (* no statement about keys being equal for now *)
-  bits_x = bits_y /\ calls_x <= length l /\ calls_y <= length l /\ v_x = v_y.
+  bits_x = bits_y /\ v_x = v_y.
+
+Theorem Gi_normal_prf_eq_compspec_post3 :
+  forall (l : list nat) (i calls : nat) (k1 k2 v : Bvector eta),
+    calls <= i ->
+    calls < length l ->
+    i < length l ->
+   comp_spec
+
+     (fun (x : list (list (Bvector eta)) * (nat * KV))
+        (y : list (list (Bvector eta)) * (nat * KV) * unit) =>
+        bitsVEq l i x y)
+
+     (oracleMap (pair_EqDec nat_EqDec eqDecState) (list_EqDec eqdbv)
+        (Oi_prg i) (calls, (k1, v)) l)
+
+     ((oracleCompMap_inner
+         (pair_EqDec (list_EqDec (list_EqDec eqdbv))
+            (pair_EqDec nat_EqDec eqDecState))
+         (list_EqDec (list_EqDec eqdbv)) (Oi_oc' i) 
+         (calls, (k2, v)) l) unit unit_EqDec (* note: k's differ. we aren't using this one *)
+        (f_oracle f eqdbv k1) tt).
+Proof.
+  intros.
+  (* NOTE: deal w/ calls increasing? *)
+  (* induction calls as [ | calls']. *)
+  (* how to get calls to increase... *)
+
+  pose (bits := @nil (list (Bvector eta))).
+  assert (H_states : bitsVEq l i (bits, (calls, (k1, v))) (bits, (calls, (k2, v)), tt)). {
+    simpl.
+    repeat (split; auto; try omega). 
+  }
+  clearbody bits.
+  clear H0.
+  clear H1.
+  
+  revert bits calls H H_states.
+  (* calls increases as l decreases *)
+  induction l as [ | x xs]; intros.
+
+  - simpl in *.
+    simplify.
+    fcf_spec_ret.
+    simpl.
+    repeat (split; auto).
+
+  -
+    simpl in H_states.
+    decompose [and] H_states; clear H_states.
+    clear H0 H1.
+
+    assert (H_ilen : calls < i \/ calls = i) by omega.
+    destruct H_ilen.
+
+Opaque Oi_prg. Opaque Oi_oc'.
+    unfold oracleMap.
+    simplify.
+    fcf_skip. admit. admit.
+    (*          |- list (Bvector eta) * (nat * KV) ->
+            list (Bvector eta) * (nat * KV) * unit -> Prop]  *)
+    instantiate (1 := (fun c d => fst c = fst (fst d) /\ snd c = snd (fst d))).
+    (* includes calls *)
+    admit.
+
+    simpl in H3. decompose [and] H3; clear H3. destruct b. destruct p. simpl in *. subst.
+    (* now need to apply induction hypothesis somehow *)
+    fcf_ident_expand_l.
+    unfold oracleMap in IHxs.
+    fcf_skip.
+    (* the fold needs to be generalized for any acc not nil (and OCM too) *)
+    (* IH does not apply for all (k2,k1,v), needs to be generalized *)
+    (* IH requires that f_oracle have same key as oracleMap when it doesn't? unsure.
+     since calls still < i, we can prove it doesn't matter *)
+    (* but other than that, this might work!! *)
+    (* apply IHxs. *)
+
+    (* old: assert (bits': list (list (Bvector eta))) by admit.
+    specialize (IHxs bits' (S calls)).
+    (* bits should be returned by... *)
+
+    assert (pre : bitsCallsVEq xs (S calls) i (bits', (S calls, (k1, v)))
+           (bits', (S calls, (k2, v)), tt)). admit.
+    admit. *)
+
+    instantiate (1 := (fun c d => bitsVEq xs i c d)).
+    admit.
+
+    simpl in H5. destruct b1. destruct b. destruct p. destruct p. destruct k. simpl in *. 
+    Ltac breakdown x := decompose [and] x; clear x.
+    breakdown H5.
+    subst.
+    simplify.
+    fcf_spec_ret. simpl.
+    repeat (split; auto).
+    (* TODO this isn't good *)
+    admit.
+    
+  +
+    clear IHxs.                 (* calls = i *)
+
+    Lemma Gi_normal_prf_eq_calls_eq_i :
+      forall (l : list nat) (i calls : nat) (k1 k2 v : Bvector eta),
+        calls >= i ->
+        comp_spec
+          (fun (x0 : list (list (Bvector eta)) * (nat * KV))
+               (y : list (list (Bvector eta)) * (nat * KV) * unit) =>
+             bitsVEq l i x0 y)
+          (oracleMap (pair_EqDec nat_EqDec eqDecState) (list_EqDec eqdbv)
+                     (Oi_prg i) (calls, (k1, v)) l)
+          ((oracleCompMap_inner
+              (pair_EqDec (list_EqDec (list_EqDec eqdbv))
+                          (pair_EqDec nat_EqDec eqDecState))
+              (list_EqDec (list_EqDec eqdbv)) (Oi_oc' i) 
+              (calls, (k2, v)) l) unit unit_EqDec 
+                                  (f_oracle f eqdbv k1) tt).
+    Proof.
+    (* pay attention to the precondition and postcondition needed here *)
+    (* but will the IH work with 'calls = i'?? it will work with calls >= i tho! condition changing... *)
+      induction l as [ | x xs]; intros.
+
+      - simplify. fcf_spec_ret. simpl. repeat (split; auto).
+      - unfold oracleMap.
+        simplify.
+        fcf_skip. admit. admit.
+        { instantiate (1 := (fun c d => fst c = fst (fst d) /\ snd c = snd (fst d))).
+        (* TODO is this true? well keys are linked so yes. don't even need calls >= i *)
+        Transparent Oi_prg. Transparent Oi_oc'.
+        unfold Oi_prg. unfold Oi_oc'.
+        simplify.
+        (* fcf_skip. admit. admit. *)
+        (* casework on `calls = i` and `calls > i` *)
+        admit. }
+
+        { simplify. simpl in *. destruct p. breakdown H2. inversion H4. subst.
+        (* possibly like before, l already entered compFold? *)
+        (* the hard case is the one-call case & the rest is just manipulation to apply IH? *)
+        (* well the base case is clearly not hard... *)
+        unfold oracleMap in *.
+
+        }
+
+
+    Admitted.
+        
+      
+      (* -------- *)
+      (* induct on reverse *)
+(*
+      remember (rev l) as rev_l.
+      assert (H_revl: rev (rev l) = l).
+      { apply rev_involutive. }
+      rewrite <- H_revl.
+      rewrite <- Heqrev_l.
+      clear Heqrev_l H_revl.
+      revert i calls k1 k2 v H.
+
+      induction rev_l as [ | rev_x' rev_l']; intros.
+
+      - unfold oracleMap.
+        simplify.
+        fcf_spec_ret.
+        simpl.
+        repeat (split; auto).
+
+      - simpl.
+        unfold oracleMap.
+        eapply comp_spec_eq_trans_l.
+        apply fold_app_2. admit. admit.
+
+        apply comp_spec_symm.
+        eapply comp_spec_eq_trans_l.
+        apply oracleCompMap_fold_app. (* is this strong enough? and fold_app_2? *)
+        apply comp_spec_symm.
+
+        fcf_skip. admit. admit.
+        
+        + apply IHrev_l'; auto.
+
+        +
+          simpl in H2. destruct b0. destruct b. repeat destruct p. destruct k. simpl in *.
+          breakdown H2. subst.
+          simplify.
+          fcf_skip. admit. admit.
+
+          Show Existentials.
+          instantiate (1 := (fun c d => fst c = fst (fst d) /\ snd c = snd (fst d))).
+    (* is this true? wait the keys are not linked... because...we don't have that postcondition on the IH. but we can add a more specific postcondition? do we need the calls stuff too? *)
+          (* or, maybe i shouldn't induct on the reverse?? *)
+          rename b2 into v'.
+          
+
+          admit.
+
+          simpl in H4. breakdown H4. destruct b1. destruct p. simpl in *. subst.
+          simplify.
+          fcf_spec_ret. simpl. destruct b3. repeat (split; auto).
+    Qed. *)
+
+    apply Gi_normal_prf_eq_calls_eq_i; omega.
+Qed.
 
 (* TODO: fix instantiations of bitsCallsKVeq below and fix postconditions
 (where there is `repeat (split; try auto))` *)
@@ -2058,72 +2258,6 @@ do i even need this?
 Admitted.
 
 (* old proof attempts *)
-(*
-  set (calls := 0).
-  (* original l = l1 ++ l2 *)
-  pose (l1 := @nil nat).
-  pose (l2 := l).
-  change l with l2 at 2 3.
-  
-  assert (H_states : bitsCallsKVeq_RB l1 l2 l i k1 k2 (@nil (list (Bvector eta)), (calls, (k1, v))) (@nil (list (Bvector eta)), (calls, (k2, v)), tt)). {
-    simpl.
-    repeat (split; auto). subst calls. omega.
-  }
-
-  change l with l2 in H.
-  clearbody l1 calls l2.
-  clear H.
-  revert calls l1 l2 H_states.
-
-  induction i as [ | i']; intros.
-
-
-  (* ------------ *)
-
-  set (calls := 0).
-  (* original l = l1 ++ l2 *)
-  pose (l1 := @nil nat).
-  pose (l2 := l).
-  change l with l2 at 2 3.
-  
-  assert (H_states : bitsCallsKVeq_RB l1 l2 l i k1 k2 (@nil (list (Bvector eta)), (calls, (k1, v))) (@nil (list (Bvector eta)), (calls, (k2, v)), tt)). {
-    simpl.
-    repeat (split; auto). subst calls. omega.
-  }
-
-  change l with l2 in H.
-  clearbody l1 calls l2.
-  clear H.
-  revert calls l1 l2 H_states.
-
-  induction i as [ | i']; intros.
-
--
-  hnf in H_states.
-  decompose [ and ] H_states; clear H_states.
-  (* destruct H_states as [? [? ?]]. *)
-  assert (H_c : calls = 0) by omega.
-  subst.
-  destruct l1; inversion H_c.
-  simpl in H.
-  clear H H0 H3 H4 H1 H_c H2.
-  rename l2 into l.
-  simpl app.
-  admit.
-  (* TODO apply lemma above w/ i = 0 *)
--
-    hnf in H_states.
-  decompose [ and ] H_states; clear H_states.
-  clear H H1 H0 H3 H4.
-  destruct l2 as [ | x l2']; inversion H8.
-
-  specialize (IHi' (S calls) (l1 ++ x :: nil) l2').
-  unfold Oi_oc'.
-
-  
-  apply IHi'. *)
-
-  (* --------- *)
 (*  destruct l as [ | x xs].
   - 
     simpl in *. omega.
@@ -2295,19 +2429,6 @@ i just don't see why you would do this, it looks worse than the oracleMap expres
 - more complicated/specific ind invariant: if calls = 0 then it returns ... else if calls > i then ... else ... and afterward calls = ... 
   still a postcondition might help for the inductive case, but won't work for the base case
 - i'm fairly sure the top-level theorem is true though!! *)
-
-(* new postcondition *)
-Definition bitsCallsVEq {A B : Type} (l : list B)
-           (x : A * (nat * KV)) (y : A * (nat * KV) * unit) :=
-  let (bits_x, state_x) := x in
-  let (calls_x, kv_x) := state_x in
-  let (k_x, v_x) := kv_x in
-
-  let (bits_y, state_y) := fst y in
-  let (calls_y, kv_y) := state_y in
-  let (k_y, v_y) := kv_y in
-  (* no statement about keys being equal for now *)
-  bits_x = bits_y /\ calls_x = length l /\ calls_y = length l /\ v_x = v_y.
 
 Theorem Gi_normal_prf_eq_compspec_post :
   forall (l : list nat) (i : nat) (k1 k2 v : Bvector eta),
